theories/lang/cpp/semantics/operator.v
@@ -265,3 +265,14 @@ Axiom eval_unop_not:
     b = bitFlipZU a (bitsN w) ->
     has_type (Vint b) (Tint w s) ->
     @eval_unop genv Ubnot (Tint w s) (Tint w s)  (Vint a) (Vint b).
+
+(** for pre- and post- increment/decrement, this function determines the type
+    of the [1] that is added or subtracted
+ *)
+Fixpoint companion_type (t : type) : option type :=
+  match t with
+  | Tpointer _ => Some (Tint int_bits Signed)
+  | Tint _ _ => Some t
+  | Tqualified _ t => companion_type t
+  | _ => None
+  end.
